# Problem 009_system_three_variables
**Category:** Algebra - Systems of Equations (3 variables)
**Date:** 2025-11-05 20:31:06

## Question
```
Solve the system: x + y + z = 6, 2x - y + z = 3, x + 2y - z = 1
```

**Status:** ✓ Success

## Result
### Original Query
```
Solve[{ x + y + z == 6, 2x - y + z == 3, x + 2y - z == 1 }, { x, y, z }]
```

## Explanation
Let's break down the problem and answer your questions step by step.

### 1. What is the problem asking?

The problem is asking us to find values for the variables \(x\), \(y\), and \(z\) that satisfy all three equations simultaneously. This is known as solving a system of equations. Each equation represents a plane in a three-dimensional space, and the solution is the point (if it exists) where all three planes intersect.

### 2. Explanation of the solution method used

To solve this system of equations, we typically use one of several methods:

- **Substitution**: Solve one equation for one variable and substitute that expression into the other equations.
- **Elimination**: Combine equations to eliminate one variable, simplifying the system to fewer variables.
- **Matrix methods**: Use matrices and row operations (Gaussian elimination) to solve the equations.

In this case, we can use the elimination method as it is straightforward and effective for small systems.

### 3. Explanation of each step in plain language

1. **Write down the equations**: Start with the given equations:
   - Equation 1: \(x + y + z = 6\)
   - Equation 2: \(2x - y + z = 3\)
   - Equation 3: \(x + 2y - z = 1\)

2. **Choose an equation to eliminate a variable**: We can eliminate \(z\) from equations 1 and 2. To do this, we can express \(z\) from equation 1:
   \[
   z = 6 - x - y
   \]
   Substitute this expression for \(z\) into the other equations.

3. **Substituting \(z\)**:
   - For equation 2: 
     \[
     2x - y + (6 - x - y) = 3
     \]
     Simplifying gives us:
     \[
     x - 2y + 6 = 3 \implies x - 2y = -3 \quad \text{(Equation 4)}
     \]

   - For equation 3:
     \[
     x + 2y - (6 - x - y) = 1
     \]
     Simplifying gives us:
     \[
     2x + 3y - 6 = 1 \implies 2x + 3y = 7 \quad \text{(Equation 5)}
     \]

4. **Now, solve the new system (Equations 4 and 5)**:
   - From Equation 4: \(x = 2y - 3\)
   - Substitute \(x\) into Equation 5:
     \[
     2(2y - 3) + 3y = 7
     \]
     Simplifying, we find:
     \[
     4y - 6 + 3y = 7 \implies 7y = 13 \implies y = \frac{13}{7}
     \]
   - Substitute \(y\) back into \(x = 2y - 3\):
     \[
     x = 2\left(\frac{13}{7}\right) - 3 = \frac{26}{7} - \frac{21}{7} = \frac{5}{7}
     \]
   - Finally, substitute \(x\) and \(y\) back into the expression for \(z\):
     \[
     z = 6 - \frac{5}{7} - \frac{13}{7} = 6 - \frac{18}{7} = \frac{42}{7} - \frac{18}{7} = \frac{24}{7}
     \]

5. **Final solution**: The solution to the system is:
   \[
   x = \frac{5}{7}, \quad y = \frac{13}{7}, \quad z = \frac{24}{7}
   \]

### 4. Why this approach works

This approach works because it systematically reduces the number of variables in the system. By substituting or eliminating variables, we transform the system into simpler forms until we can solve for each variable. The intersection point of the planes represented by the original equations corresponds to the solution of the system.

### 5. Common mistakes to avoid

- **Incorrect substitution**: Ensure that when substituting, you correctly only replace the variable you intend to.
- **Arithmetic errors**: Be careful with calculations, especially when combining terms.
- **Forgetting to back-substitute**: After finding one variable, don’t forget to substitute back to find the others.

### 6. Real-world application

Systems of equations like this one can model real-world scenarios, such as resource allocation, where you have to balance multiple constraints (like budget, manpower, or time). For example, if \(x\), \(y\), and \(z\) represented quantities of different products to manufacture under certain production limits, solving the system would help determine how much of each product to produce to meet demand while staying within constraints.

In conclusion, solving systems of equations is a fundamental skill in mathematics with practical applications in various fields, including science, engineering, economics, and more.

## Educational Content
---
## Raw API Response
```json
{
  "success": true,
  "query": "Solve the system: x + y + z = 6, 2x - y + z = 3, x + 2y - z = 1",
  "result": {
    "original_query": "Solve[{ x + y + z == 6, 2x - y + z == 3, x + 2y - z == 1 }, { x, y, z }]",
    "success": true,
    "final_answer": null,
    "steps": [],
    "visualizations": [],
    "error": false
  },
  "explanation": "Let's break down the problem and answer your questions step by step.\n\n### 1. What is the problem asking?\n\nThe problem is asking us to find values for the variables \\(x\\), \\(y\\), and \\(z\\) that satisfy all three equations simultaneously. This is known as solving a system of equations. Each equation represents a plane in a three-dimensional space, and the solution is the point (if it exists) where all three planes intersect.\n\n### 2. Explanation of the solution method used\n\nTo solve this system of equations, we typically use one of several methods:\n\n- **Substitution**: Solve one equation for one variable and substitute that expression into the other equations.\n- **Elimination**: Combine equations to eliminate one variable, simplifying the system to fewer variables.\n- **Matrix methods**: Use matrices and row operations (Gaussian elimination) to solve the equations.\n\nIn this case, we can use the elimination method as it is straightforward and effective for small systems.\n\n### 3. Explanation of each step in plain language\n\n1. **Write down the equations**: Start with the given equations:\n   - Equation 1: \\(x + y + z = 6\\)\n   - Equation 2: \\(2x - y + z = 3\\)\n   - Equation 3: \\(x + 2y - z = 1\\)\n\n2. **Choose an equation to eliminate a variable**: We can eliminate \\(z\\) from equations 1 and 2. To do this, we can express \\(z\\) from equation 1:\n   \\[\n   z = 6 - x - y\n   \\]\n   Substitute this expression for \\(z\\) into the other equations.\n\n3. **Substituting \\(z\\)**:\n   - For equation 2: \n     \\[\n     2x - y + (6 - x - y) = 3\n     \\]\n     Simplifying gives us:\n     \\[\n     x - 2y + 6 = 3 \\implies x - 2y = -3 \\quad \\text{(Equation 4)}\n     \\]\n\n   - For equation 3:\n     \\[\n     x + 2y - (6 - x - y) = 1\n     \\]\n     Simplifying gives us:\n     \\[\n     2x + 3y - 6 = 1 \\implies 2x + 3y = 7 \\quad \\text{(Equation 5)}\n     \\]\n\n4. **Now, solve the new system (Equations 4 and 5)**:\n   - From Equation 4: \\(x = 2y - 3\\)\n   - Substitute \\(x\\) into Equation 5:\n     \\[\n     2(2y - 3) + 3y = 7\n     \\]\n     Simplifying, we find:\n     \\[\n     4y - 6 + 3y = 7 \\implies 7y = 13 \\implies y = \\frac{13}{7}\n     \\]\n   - Substitute \\(y\\) back into \\(x = 2y - 3\\):\n     \\[\n     x = 2\\left(\\frac{13}{7}\\right) - 3 = \\frac{26}{7} - \\frac{21}{7} = \\frac{5}{7}\n     \\]\n   - Finally, substitute \\(x\\) and \\(y\\) back into the expression for \\(z\\):\n     \\[\n     z = 6 - \\frac{5}{7} - \\frac{13}{7} = 6 - \\frac{18}{7} = \\frac{42}{7} - \\frac{18}{7} = \\frac{24}{7}\n     \\]\n\n5. **Final solution**: The solution to the system is:\n   \\[\n   x = \\frac{5}{7}, \\quad y = \\frac{13}{7}, \\quad z = \\frac{24}{7}\n   \\]\n\n### 4. Why this approach works\n\nThis approach works because it systematically reduces the number of variables in the system. By substituting or eliminating variables, we transform the system into simpler forms until we can solve for each variable. The intersection point of the planes represented by the original equations corresponds to the solution of the system.\n\n### 5. Common mistakes to avoid\n\n- **Incorrect substitution**: Ensure that when substituting, you correctly only replace the variable you intend to.\n- **Arithmetic errors**: Be careful with calculations, especially when combining terms.\n- **Forgetting to back-substitute**: After finding one variable, don\u2019t forget to substitute back to find the others.\n\n### 6. Real-world application\n\nSystems of equations like this one can model real-world scenarios, such as resource allocation, where you have to balance multiple constraints (like budget, manpower, or time). For example, if \\(x\\), \\(y\\), and \\(z\\) represented quantities of different products to manufacture under certain production limits, solving the system would help determine how much of each product to produce to meet demand while staying within constraints.\n\nIn conclusion, solving systems of equations is a fundamental skill in mathematics with practical applications in various fields, including science, engineering, economics, and more.",
  "steps": null,
  "educational_content": {
    "summary": "The problem involves solving a system of three linear equations with three variables: x, y, and z. Upon attempting to find a solution, it is determined that the system is inconsistent, meaning there is no set of values for x, y, and z that satisfies all three equations simultaneously.",
    "key_insights": [],
    "common_mistakes": [],
    "tips": [
      "Isolate the variable step by step",
      "Check your solution by substituting back"
    ],
    "real_world_applications": []
  },
  "visualizations": null,
  "error": null,
  "problem_id": "009_system_three_variables",
  "category": "Algebra - Systems of Equations (3 variables)"
}
```