# Problem 013_logarithm
**Category:** Algebra - Logarithmic Equations
**Date:** 2025-11-05 20:32:20

## Question
```
Solve log(x) + log(x-3) = 1
```

**Status:** âœ“ Success

## Result
### Final Answer
```latex
we can rewrite the equation as:
```

### Original Query
```
Solve log(x) + log(x-3) = 1
```

## Step-by-Step Solution
### Step 3
**Description:** = 1 \), we will follow a structured approach.

```latex
= 1 \), we will follow a structured approach.
```

### Step 3
**Description:** = \log(x(x-

```latex
= \log(x(x-
```

### Step 3
**Description:** )

```latex
)
```

### Step 3
**Description:** ) = 1

```latex
) = 1
```

### Step 10
**Description:** . Therefore, we have:

```latex
. Therefore, we have:
```

### Step 3
**Description:** = 10^1

```latex
= 10^1
```

### Step 3
**Description:** = 10

```latex
= 10
```

### Step 3
**Description:** \pm \sqrt{(-

```latex
\pm \sqrt{(-
```

### Step 3
**Description:** ^2 - 4 \cdot 1 \cdot (-

```latex
^2 - 4 \cdot 1 \cdot (-
```

### Step 10
**Description:** }}{2 \cdot 1}

```latex
}}{2 \cdot 1}
```

## Explanation
To solve the equation \( \log(x) + \log(x-3) = 1 \), we will follow a structured approach. 

### Step 1: Use Properties of Logarithms

First, we can use the property of logarithms that states \( \log(a) + \log(b) = \log(ab) \). Applying this property to our equation, we get:

\[
\log(x) + \log(x-3) = \log(x(x-3))
\]

Thus, we can rewrite the equation as:

\[
\log(x(x-3)) = 1
\]

### Step 2: Exponentiate Both Sides

To eliminate the logarithm, we exponentiate both sides of the equation. Recall that if \( \log(a) = b \), then \( a = 10^b \) (assuming the logarithm is base 10). Therefore, we have:

\[
x(x-3) = 10^1
\]

This simplifies to:

\[
x(x-3) = 10
\]

### Step 3: Expand and Rearrange

Next, we expand the left-hand side:

\[
x^2 - 3x = 10
\]

Now, we rearrange the equation to set it to zero:

\[
x^2 - 3x - 10 = 0
\]

### Step 4: Solve the Quadratic Equation

We will solve the quadratic equation \( x^2 - 3x - 10 = 0 \) using the quadratic formula:

\[
x = \frac{-b \pm \sqrt{b^2 - 4ac}}{2a}
\]

Here, \( a = 1 \), \( b = -3 \), and \( c = -10 \). Plugging in these values:

\[
x = \frac{-(-3) \pm \sqrt{(-3)^2 - 4 \cdot 1 \cdot (-10)}}{2 \cdot 1}
\]

Calculating the discriminant:

\[
(-3)^2 - 4 \cdot 1 \cdot (-10) = 9 + 40 = 49
\]

Now substituting back into the formula:

\[
x = \frac{3 \pm \sqrt{49}}{2}
\]

Since \( \sqrt{49} = 7 \), we have:

\[
x = \frac{3 \pm 7}{2}
\]

This gives us two potential solutions:

1. \( x = \frac{10}{2} = 5 \)
2. \( x = \frac{-4}{2} = -2 \)

### Step 5: Check for Validity of Solutions

Since we are dealing with logarithms, we need to ensure that the arguments of the logarithmic functions are positive. 

1. For \( x = 5 \):
   - \( x - 3 = 5 - 3 = 2 \) (valid since both \( x \) and \( x-3 \) are positive)

2. For \( x = -2 \):
   - \( x - 3 = -2 - 3 = -5 \) (invalid since \( x-3 \) is negative)

Thus, the only valid solution is \( x = 5 \).

### Final Answer

The solution to the equation \( \log(x) + \log(x-3) = 1 \) is:

\[
\boxed{5}
\]

### Explanation of Key Concepts Used

1. **Properties of Logarithms**: We used the property that the sum of logarithms is the logarithm of the product. This is crucial for simplifying logarithmic equations.
  
2. **Quadratic Formula**: This formula provides a systematic way to find the roots of any quadratic equation, which is essential when the equation cannot be factored easily.

3. **Domain Considerations**: When dealing with logarithmic functions, it is important to check that the arguments of the logarithms are positive, as logarithms are only defined for positive numbers.

### Relevant Mathematical Insights

- Logarithmic equations often require careful manipulation and understanding of their properties. 
- Quadratic equations can arise from various mathematical contexts, and the quadratic formula is a powerful tool for finding solutions.
- Always consider the domain of the functions involved when solving equations, especially with logarithmic and radical expressions.

## Educational Content
---
## Raw API Response
```json
{
  "success": true,
  "query": "Solve log(x) + log(x-3) = 1",
  "result": {
    "success": true,
    "original_query": "Solve log(x) + log(x-3) = 1",
    "final_answer": "we can rewrite the equation as:",
    "explanation": "To solve the equation \\( \\log(x) + \\log(x-3) = 1 \\), we will follow a structured approach. \n\n### Step 1: Use Properties of Logarithms\n\nFirst, we can use the property of logarithms that states \\( \\log(a) + \\log(b) = \\log(ab) \\). Applying this property to our equation, we get:\n\n\\[\n\\log(x) + \\log(x-3) = \\log(x(x-3))\n\\]\n\nThus, we can rewrite the equation as:\n\n\\[\n\\log(x(x-3)) = 1\n\\]\n\n### Step 2: Exponentiate Both Sides\n\nTo eliminate the logarithm, we exponentiate both sides of the equation. Recall that if \\( \\log(a) = b \\), then \\( a = 10^b \\) (assuming the logarithm is base 10). Therefore, we have:\n\n\\[\nx(x-3) = 10^1\n\\]\n\nThis simplifies to:\n\n\\[\nx(x-3) = 10\n\\]\n\n### Step 3: Expand and Rearrange\n\nNext, we expand the left-hand side:\n\n\\[\nx^2 - 3x = 10\n\\]\n\nNow, we rearrange the equation to set it to zero:\n\n\\[\nx^2 - 3x - 10 = 0\n\\]\n\n### Step 4: Solve the Quadratic Equation\n\nWe will solve the quadratic equation \\( x^2 - 3x - 10 = 0 \\) using the quadratic formula:\n\n\\[\nx = \\frac{-b \\pm \\sqrt{b^2 - 4ac}}{2a}\n\\]\n\nHere, \\( a = 1 \\), \\( b = -3 \\), and \\( c = -10 \\). Plugging in these values:\n\n\\[\nx = \\frac{-(-3) \\pm \\sqrt{(-3)^2 - 4 \\cdot 1 \\cdot (-10)}}{2 \\cdot 1}\n\\]\n\nCalculating the discriminant:\n\n\\[\n(-3)^2 - 4 \\cdot 1 \\cdot (-10) = 9 + 40 = 49\n\\]\n\nNow substituting back into the formula:\n\n\\[\nx = \\frac{3 \\pm \\sqrt{49}}{2}\n\\]\n\nSince \\( \\sqrt{49} = 7 \\), we have:\n\n\\[\nx = \\frac{3 \\pm 7}{2}\n\\]\n\nThis gives us two potential solutions:\n\n1. \\( x = \\frac{10}{2} = 5 \\)\n2. \\( x = \\frac{-4}{2} = -2 \\)\n\n### Step 5: Check for Validity of Solutions\n\nSince we are dealing with logarithms, we need to ensure that the arguments of the logarithmic functions are positive. \n\n1. For \\( x = 5 \\):\n   - \\( x - 3 = 5 - 3 = 2 \\) (valid since both \\( x \\) and \\( x-3 \\) are positive)\n\n2. For \\( x = -2 \\):\n   - \\( x - 3 = -2 - 3 = -5 \\) (invalid since \\( x-3 \\) is negative)\n\nThus, the only valid solution is \\( x = 5 \\).\n\n### Final Answer\n\nThe solution to the equation \\( \\log(x) + \\log(x-3) = 1 \\) is:\n\n\\[\n\\boxed{5}\n\\]\n\n### Explanation of Key Concepts Used\n\n1. **Properties of Logarithms**: We used the property that the sum of logarithms is the logarithm of the product. This is crucial for simplifying logarithmic equations.\n  \n2. **Quadratic Formula**: This formula provides a systematic way to find the roots of any quadratic equation, which is essential when the equation cannot be factored easily.\n\n3. **Domain Considerations**: When dealing with logarithmic functions, it is important to check that the arguments of the logarithms are positive, as logarithms are only defined for positive numbers.\n\n### Relevant Mathematical Insights\n\n- Logarithmic equations often require careful manipulation and understanding of their properties. \n- Quadratic equations can arise from various mathematical contexts, and the quadratic formula is a powerful tool for finding solutions.\n- Always consider the domain of the functions involved when solving equations, especially with logarithmic and radical expressions.",
    "steps": [
      {
        "step_number": 3,
        "description": "= 1 \\), we will follow a structured approach.",
        "math": "= 1 \\), we will follow a structured approach."
      },
      {
        "step_number": 3,
        "description": "= \\log(x(x-",
        "math": "= \\log(x(x-"
      },
      {
        "step_number": 3,
        "description": ")",
        "math": ")"
      },
      {
        "step_number": 3,
        "description": ") = 1",
        "math": ") = 1"
      },
      {
        "step_number": 10,
        "description": ". Therefore, we have:",
        "math": ". Therefore, we have:"
      },
      {
        "step_number": 3,
        "description": "= 10^1",
        "math": "= 10^1"
      },
      {
        "step_number": 3,
        "description": "= 10",
        "math": "= 10"
      },
      {
        "step_number": 3,
        "description": "\\pm \\sqrt{(-",
        "math": "\\pm \\sqrt{(-"
      },
      {
        "step_number": 3,
        "description": "^2 - 4 \\cdot 1 \\cdot (-",
        "math": "^2 - 4 \\cdot 1 \\cdot (-"
      },
      {
        "step_number": 10,
        "description": "}}{2 \\cdot 1}",
        "math": "}}{2 \\cdot 1}"
      }
    ],
    "educational_content": {
      "summary": "This is a undergraduate-level mathematical problem.",
      "key_insights": [],
      "common_mistakes": [],
      "tips": [],
      "real_world_applications": []
    },
    "visualizations": [],
    "error": null
  },
  "explanation": "To solve the equation \\( \\log(x) + \\log(x-3) = 1 \\), we will follow a structured approach. \n\n### Step 1: Use Properties of Logarithms\n\nFirst, we can use the property of logarithms that states \\( \\log(a) + \\log(b) = \\log(ab) \\). Applying this property to our equation, we get:\n\n\\[\n\\log(x) + \\log(x-3) = \\log(x(x-3))\n\\]\n\nThus, we can rewrite the equation as:\n\n\\[\n\\log(x(x-3)) = 1\n\\]\n\n### Step 2: Exponentiate Both Sides\n\nTo eliminate the logarithm, we exponentiate both sides of the equation. Recall that if \\( \\log(a) = b \\), then \\( a = 10^b \\) (assuming the logarithm is base 10). Therefore, we have:\n\n\\[\nx(x-3) = 10^1\n\\]\n\nThis simplifies to:\n\n\\[\nx(x-3) = 10\n\\]\n\n### Step 3: Expand and Rearrange\n\nNext, we expand the left-hand side:\n\n\\[\nx^2 - 3x = 10\n\\]\n\nNow, we rearrange the equation to set it to zero:\n\n\\[\nx^2 - 3x - 10 = 0\n\\]\n\n### Step 4: Solve the Quadratic Equation\n\nWe will solve the quadratic equation \\( x^2 - 3x - 10 = 0 \\) using the quadratic formula:\n\n\\[\nx = \\frac{-b \\pm \\sqrt{b^2 - 4ac}}{2a}\n\\]\n\nHere, \\( a = 1 \\), \\( b = -3 \\), and \\( c = -10 \\). Plugging in these values:\n\n\\[\nx = \\frac{-(-3) \\pm \\sqrt{(-3)^2 - 4 \\cdot 1 \\cdot (-10)}}{2 \\cdot 1}\n\\]\n\nCalculating the discriminant:\n\n\\[\n(-3)^2 - 4 \\cdot 1 \\cdot (-10) = 9 + 40 = 49\n\\]\n\nNow substituting back into the formula:\n\n\\[\nx = \\frac{3 \\pm \\sqrt{49}}{2}\n\\]\n\nSince \\( \\sqrt{49} = 7 \\), we have:\n\n\\[\nx = \\frac{3 \\pm 7}{2}\n\\]\n\nThis gives us two potential solutions:\n\n1. \\( x = \\frac{10}{2} = 5 \\)\n2. \\( x = \\frac{-4}{2} = -2 \\)\n\n### Step 5: Check for Validity of Solutions\n\nSince we are dealing with logarithms, we need to ensure that the arguments of the logarithmic functions are positive. \n\n1. For \\( x = 5 \\):\n   - \\( x - 3 = 5 - 3 = 2 \\) (valid since both \\( x \\) and \\( x-3 \\) are positive)\n\n2. For \\( x = -2 \\):\n   - \\( x - 3 = -2 - 3 = -5 \\) (invalid since \\( x-3 \\) is negative)\n\nThus, the only valid solution is \\( x = 5 \\).\n\n### Final Answer\n\nThe solution to the equation \\( \\log(x) + \\log(x-3) = 1 \\) is:\n\n\\[\n\\boxed{5}\n\\]\n\n### Explanation of Key Concepts Used\n\n1. **Properties of Logarithms**: We used the property that the sum of logarithms is the logarithm of the product. This is crucial for simplifying logarithmic equations.\n  \n2. **Quadratic Formula**: This formula provides a systematic way to find the roots of any quadratic equation, which is essential when the equation cannot be factored easily.\n\n3. **Domain Considerations**: When dealing with logarithmic functions, it is important to check that the arguments of the logarithms are positive, as logarithms are only defined for positive numbers.\n\n### Relevant Mathematical Insights\n\n- Logarithmic equations often require careful manipulation and understanding of their properties. \n- Quadratic equations can arise from various mathematical contexts, and the quadratic formula is a powerful tool for finding solutions.\n- Always consider the domain of the functions involved when solving equations, especially with logarithmic and radical expressions.",
  "steps": [
    {
      "step_number": 3,
      "description": "= 1 \\), we will follow a structured approach.",
      "math": "= 1 \\), we will follow a structured approach."
    },
    {
      "step_number": 3,
      "description": "= \\log(x(x-",
      "math": "= \\log(x(x-"
    },
    {
      "step_number": 3,
      "description": ")",
      "math": ")"
    },
    {
      "step_number": 3,
      "description": ") = 1",
      "math": ") = 1"
    },
    {
      "step_number": 10,
      "description": ". Therefore, we have:",
      "math": ". Therefore, we have:"
    },
    {
      "step_number": 3,
      "description": "= 10^1",
      "math": "= 10^1"
    },
    {
      "step_number": 3,
      "description": "= 10",
      "math": "= 10"
    },
    {
      "step_number": 3,
      "description": "\\pm \\sqrt{(-",
      "math": "\\pm \\sqrt{(-"
    },
    {
      "step_number": 3,
      "description": "^2 - 4 \\cdot 1 \\cdot (-",
      "math": "^2 - 4 \\cdot 1 \\cdot (-"
    },
    {
      "step_number": 10,
      "description": "}}{2 \\cdot 1}",
      "math": "}}{2 \\cdot 1}"
    }
  ],
  "educational_content": {
    "summary": "This is a undergraduate-level mathematical problem.",
    "key_insights": [],
    "common_mistakes": [],
    "tips": [],
    "real_world_applications": []
  },
  "visualizations": [],
  "error": null,
  "problem_id": "013_logarithm",
  "category": "Algebra - Logarithmic Equations"
}
```